\paragraph{a}
We have to prove the following equation:
\begin{equation*}
    S^{k}_{n}(A \cup B) = S^{k}_{n}(S^{k}_{n}(A) \cup S^{k}_{n}(B))\\
\end{equation*}

To do that we start by showing:
\begin{equation*}
    S^{k}_{n}(A \cup B) \supseteq S^{k}_{n}(S^{k}_{n}(A) \cup S^{k}_{n}(B))\\
\end{equation*}

We assume that we have the list A and B where the elements are sorted after the
hashed values. Then when we want to get $S^{k}_{n}(A\cup B)$ we want to take
the first $i$ elements in A and the first $k-i$ elements in B where $i$.
\begin{align*}
    A &=\{a_1, a_2, \dots , a_{i}, a_{i+1} \dots  , a_n\}\\
    B &=\{b_1, b_2, \dots , b_{k-i}, \dots , b_m\}
    S^{k}_{n}(A\cup B) =\{a_1, a_2, \dots , a_{i}, \dots,  b_1, b_2, \dots , b_{k-i-1}\}
\end{align*}

On the right side we get:
\begin{align*}
    A' &= S^{k}_{n}(A) = (\{a_1, a_2, \dots , a_{i}, a_{n}\}\\
    B' &= S^{k}_{n}(B) = \{b_1, b_2, \dots , b_{i-k}\}
\end{align*}
We then get:
\begin{equation*}
    S^{k}_{n}(A' \cup B')
\end{equation*}
Here we see:
\begin{align*}
    A &\supseteq A'\\
    B &\supseteq B'\\
    |A'| &= k\\
    |B'| &= k
\end{align*}
When we have this it is trivial to see that they are same.
