\subsection*{4b}

\begin{align*}
    A \cap B \cap S^{k}_{n}(A \cup B) &= S^{k}_{n}(A) \cap S^{k}_{n}(B) \cap S^{k}_{n}(A \cup B)\\
    &\supseteq
\end{align*}

\begin{align*}
    A &=\{a_1, a_2, \dots , a_{i}, a_{i+1} \dots  , a_n\}\\
    B &=\{b_1, b_2, \dots , b_{k-i}, \dots , b_m\}
\end{align*}

\begin{equation*}
    S^{k}_{n}(A\cup B) =\{a_1, a_2, \dots , a_{i}, b_1, b_2, \dots , b_{k-i-1}\}
\end{equation*}

\begin{equation*}
    A \cap B = \{ a | a \in A, b \in B, a = b\}
\end{equation*}

\begin{equation*}
    S^{k}_{n}(A) \cap S^{k}_{n}(B) = \{a | a \in A, b \in B, a = b, a_{pos} \le i, b_{pos} < k-i\}
\end{equation*}

$a_{pos} > i$ $b_{pos} \ge k-i$
